Write a mostly unspecified Specification

specs/x86/MCH/MCH.v
@@ -2,16 +2,104 @@ Require Import FreeSpec.Specs.x86.MCH.SMRAMC.
 Require Import FreeSpec.Specs.Memory.
 Require Import FreeSpec.Specs.Address.
 Require Import FreeSpec.Interface.
+Require Import FreeSpec.Undefined.
+Require Import FreeSpec.Refine.
+Require Import FreeSpec.Control.
+Require Import FreeSpec.Control.Classes.
+Require Import FreeSpec.Control.State.
+Require Import FreeSpec.Program.
+Require Import FreeSpec.WEq.
+Require Import FreeSpec.Compose.
+
+Local Open Scope free_scope.
+Local Open Scope free_control_scope.
+
+(** * Interface
+
+ *)
 
 Inductive MCHi
   : Interface :=
-| PIO_in (port: word)
-  : MCHi byte
-| PIO_out (port: word)
-          (val:  byte)
+| PIO_in32 (port: word)
+  : MCHi lword
+| PIO_out32 (port: word)
+            (val:  lword)
   : MCHi unit
 | IO_read (addr: address_64B_aligned)
   : MCHi (mem (64 Bytes))
 | IO_write (addr: address_64B_aligned)
            (val:  mem (64 Bytes))
   : MCHi unit.
+
+(** * Hardware Specification
+
+ *)
+
+Inductive ConfAddr
+  : Type :=
+| confaddr (bus:      nat)
+           (device:   nat)
+           (function: nat)
+           (register: nat)
+  : ConfAddr.
+
+Axiom lword_to_confaddr
+  : lword -> option ConfAddr.
+Axiom confaddr_location
+  : word.
+
+Inductive io_write32_target
+  : Type :=
+| ConfAddr_tar
+| Invalid_tar.
+
+Axiom word_to_target
+  : word -> option io_write32_target.
+
+Record MCHs :=
+  { confAddr: ConfAddr
+  }.
+
+Instance mchs_WEq
+  : WEq MCHs :=
+  { weq := eq
+  }.
+
+(** We need a notation here. If you use a plain ~Definition~, Coq
+    cannot find the typeclass instance any longer.
+
+ *)
+Notation "'MCHm' A":= (StateT MCHs (Program (MCHi <+> Undefined)) A)
+                        (at level 30).
+
+(* We have to help a little Coq here. See #16 for more information on
+   this matter *)
+Definition mch_undefined
+           {A: Type}
+  : MCHm A :=
+  undef (UndefMonad:=undefmonad_Trans _ _).
+
+Definition pio_out32
+           (x: word)
+           (val: lword)
+  : MCHm unit :=
+  match word_to_target x with
+  | Some ConfAddr_tar
+    => pure tt
+  | Some _ (* This is a valid target, but it has not been specified
+              yet                                                   *)
+    => mch_undefined
+  | Nothing (* An invalid IO out access is just ignore by the MCH   *)
+    => pure tt
+  end.
+
+Definition mch_specs
+  : StatefulRefinement MCHi (MCHi <+> Undefined) MCHs :=
+  fun (A: Type)
+      (i: MCHi A)
+  => match i with
+     | PIO_out32 x val
+       => pio_out32 x val
+     | _
+       => mch_undefined
+     end.
